ReTierProofAggregation.v
@@ -6,46 +6,51 @@ Lemma aggregation_multiple : forall
     (c: context)
     (p0 p1 : P)
     (peers: Coq.Lists.ListSet.set p)
-    (term: t)
-    (value: t)
-    (value_type: T),
+    (v v_agg: t)
+    (v_type: T),
   getTieMult c (p0, p1) = Some multiple ->
-  c |- value \in value_type ->
-  Phi (getTies c) p0 p1 peers value value_type = Some term ->
-  c |- term \in (List value_type).
+  transmittable_value v ->
+  c |- v \in v_type ->
+  Phi (getTies c) p0 p1 peers v v_type = Some v_agg ->
+  transmittable_value v_agg /\ c |- v_agg \in (List v_type).
 Proof.
-intros c p0 p1 peers term value value_type.
-intros H_multiple H_value_type H_Phi_term.
+intros until v_type.
+intros H_multiple H_value H_v_type H_Phi.
 unfold getTieMult in H_multiple.
-generalize dependent term.
-induction peers as [| peer0 peers IH_peers ]; intros term H_Phi_term.
-- simpl in H_Phi_term.
-  rewrite H_multiple in H_Phi_term.
-  inversion H_Phi_term.
-  apply T_Nil.
-- assert (H : exists term, Phi (getTies c) p0 p1 peers value value_type = Some term).
-  + clear IH_peers H_Phi_term.
+generalize dependent v_agg.
+induction peers as [| peer0 peers IH_peers ]; intros v_agg H_Phi.
+- simpl in H_Phi.
+  rewrite H_multiple in H_Phi.
+  inversion H_Phi.
+  split.
+  + apply w_nil.
+  + apply T_Nil.
+- assert (H : exists v_agg, Phi (getTies c) p0 p1 peers v v_type = Some v_agg).
+  + clear IH_peers H_Phi.
     induction peers as [| peer1 peers IH_peers ].
     * simpl.
       rewrite H_multiple.
-      exists (nil value_type).
+      exists (nil v_type).
       reflexivity.
     * simpl.
       rewrite H_multiple.
-      inversion IH_peers as [ term2 H_Phi_term2 ].
-      rewrite H_Phi_term2.
-      exists (cons value term2).
+      inversion IH_peers as [ v_agg2 H_Phi2 ].
+      rewrite H_Phi2.
+      exists (cons v v_agg2).
       reflexivity.
-  + inversion H as [ term2 H_Phi_term2 ].
-    simpl in IH_peers, H_Phi_term, H_Phi_term2.
-    rewrite H_multiple in H_Phi_term.
-    rewrite H_Phi_term2 in H_Phi_term.
-    rewrite H_Phi_term2 in IH_peers.
-    clear H_Phi_term2.
-    inversion H_Phi_term.
-    apply T_Cons.
-    * assumption.
-    * apply IH_peers.
+  + inversion H as [ v_agg2 H_Phi2 ].
+    simpl in IH_peers, H_Phi, H_Phi2.
+    rewrite H_multiple in H_Phi.
+    rewrite H_Phi2 in H_Phi.
+    rewrite H_Phi2 in IH_peers.
+    clear H_Phi2.
+    inversion H_Phi.
+    split.
+    * apply w_cons; try assumption.
+      apply IH_peers.
+      reflexivity.
+    * apply T_Cons; try assumption.
+      apply IH_peers.
       reflexivity.
 Qed.
 
@@ -53,29 +58,32 @@ Lemma aggregation_optional : forall
     (c: context)
     (p0 p1 : P)
     (peers: Coq.Lists.ListSet.set p)
-    (term: t)
-    (value: t)
-    (value_type: T),
+    (v v_agg: t)
+    (v_type: T),
   getTieMult c (p0, p1) = Some optional ->
-  c |- value \in value_type ->
-  Phi (getTies c) p0 p1 peers value value_type = Some term ->
-  c |- term \in (Option value_type).
+  transmittable_value v ->
+  c |- v \in v_type ->
+  Phi (getTies c) p0 p1 peers v v_type = Some v_agg ->
+  transmittable_value v_agg /\ c |- v_agg \in (Option v_type).
 Proof.
-intros c p0 p1 peers term value value_type.
-intros H_multiple H_value_type H_Phi_term.
+intros until v_type.
+intros H_multiple H_value H_v_type H_Phi.
 unfold getTieMult in H_multiple.
 destruct peers.
-- simpl in H_Phi_term.
-  rewrite H_multiple in H_Phi_term.
-  inversion H_Phi_term.
-  apply T_None.
-- simpl in H_Phi_term.
-  rewrite H_multiple in H_Phi_term.
+- simpl in H_Phi.
+  rewrite H_multiple in H_Phi.
+  inversion H_Phi.
+  split.
+  + apply w_none.
+  + apply T_None.
+- simpl in H_Phi.
+  rewrite H_multiple in H_Phi.
   destruct peers.
-  + inversion H_Phi_term.
-    apply T_Some.
-    assumption.
-  + contradict H_Phi_term.
+  + inversion H_Phi.
+    split.
+    * apply w_some. assumption.
+    * apply T_Some. assumption.
+  + contradict H_Phi.
     congruence.
 Qed.
 
@@ -83,28 +91,29 @@ Lemma aggregation_single : forall
     (c: context)
     (p0 p1 : P)
     (peers: Coq.Lists.ListSet.set p)
-    (term: t)
-    (value: t)
-    (value_type: T),
+    (v v_agg: t)
+    (v_type: T),
   getTieMult c (p0, p1) = Some single ->
-  c |- value \in value_type ->
-  Phi (getTies c) p0 p1 peers value value_type = Some term ->
-  c |- term \in value_type.
+  transmittable_value v ->
+  c |- v \in v_type ->
+  Phi (getTies c) p0 p1 peers v v_type = Some v_agg ->
+  transmittable_value v_agg /\ c |- v_agg \in v_type.
 Proof.
-intros c p0 p1 peers term value value_type.
-intros H_multiple H_value_type H_Phi_term.
+intros until v_type.
+intros H_multiple H_value H_v_type H_Phi.
 unfold getTieMult in H_multiple.
 destruct peers.
-- simpl in H_Phi_term.
-  rewrite H_multiple in H_Phi_term.
-  contradict H_Phi_term.
+- simpl in H_Phi.
+  rewrite H_multiple in H_Phi.
+  contradict H_Phi.
   congruence.
-- simpl in H_Phi_term.
-  rewrite H_multiple in H_Phi_term.
+- simpl in H_Phi.
+  rewrite H_multiple in H_Phi.
   destruct peers.
-  + inversion H_Phi_term.
-    congruence.
-  + contradict H_Phi_term.
+  + inversion H_Phi.
+    subst.
+    split; assumption.
+  + contradict H_Phi.
     congruence.
 Qed.
 
@@ -112,24 +121,23 @@ Lemma aggregation : forall
     (c: context)
     (p0 p1 : P)
     (peers: Coq.Lists.ListSet.set p)
-    (value: t)
-    (value_type: T)
-    (term: t)
-    (term_type: T),
+    (v v_agg: t)
+    (v_type v_agg_type: T),
   getTieMult c (p0, p1) <> None ->
   getTieMult c (p0, p1) <> Some mNone ->
-  Phi (getTies c) p0 p1 peers value value_type = Some term ->
-  phi c p0 p1 value_type = Some term_type ->
-  c |- value \in value_type ->
-  c |- term \in term_type.
+  Phi (getTies c) p0 p1 peers v v_type = Some v_agg ->
+  phi c p0 p1 v_type = Some v_agg_type ->
+  transmittable_value v ->
+  c |- v \in v_type ->
+  transmittable_value v_agg /\ c |- v_agg \in v_agg_type.
 Proof.
-intros c p0 p1 peers value value_type term term_type.
-intros H_tie0 H_tie1 H_Phi_term H_phi_term_type H_value_type.
+intros until v_agg_type.
+intros H_tie0 H_tie1 H_Phi H_phi_type H_value H_v_type.
 case_eq (getTieMult c (p0, p1)).
 - intros multiplicity H_tie.
-  unfold phi in H_phi_term_type.
-  rewrite H_tie in H_phi_term_type.
-  destruct multiplicity; inversion H_phi_term_type as [ H_term_type ]; subst.
+  unfold phi in H_phi_type.
+  rewrite H_tie in H_phi_type.
+  destruct multiplicity; inversion H_phi_type as [ H_type ]; subst.
   + eapply aggregation_multiple; eassumption.
   + eapply aggregation_optional; eassumption.
   + eapply aggregation_single; eassumption.
