ReTierStaticSemantics.v
@@ -231,6 +231,7 @@ Inductive has_type : context -> t -> T -> Prop :=
 
         | T_AsLocal: forall context,
                      forall P0 P1 t T0 T1,
+            transmittable_type T1 ->
             (P0 = (getPeer context)) ->   (* just for better readability *)
             (remoteContext P1 context) |- t \in T1 ->
             (areTied context P0 P1) = true ->
@@ -239,6 +240,7 @@ Inductive has_type : context -> t -> T -> Prop :=
 
         | T_AsLocalFrom: forall context,
                          forall P0 P1 t0 t1 T,
+            transmittable_type T ->
             (P0 = (getPeer context)) ->   (* just for better readability *)
             (remoteContext P1 context) |- t0 \in T ->
             (areTied context P0 P1) = true ->
@@ -247,6 +249,7 @@ Inductive has_type : context -> t -> T -> Prop :=
 
         | T_Comp: forall context,
                   forall x t0 t1 T0 T1 T2 P0 P1,
+            transmittable_type T1 ->
             (P0 = (getPeer context)) ->   (* just for better readability *)
             context |- t0 \in T0 ->
             (remoteContextWithBinding P1 x T0 context) |- t1 \in T1 ->
@@ -256,6 +259,7 @@ Inductive has_type : context -> t -> T -> Prop :=
 
         | T_ComFrom:  forall context,
                       forall x t0 t1 t2 T0 T1 P0 P1,
+            transmittable_type T1 ->
             (P0 = (getPeer context)) ->   (* just for better readability *)
             context |- t0 \in T0 ->
             (remoteContextWithBinding P1 x T0 context) |- t1 \in T1 ->
